fix W

Logic/Vorspiel/W.lean
@@ -5,25 +5,15 @@ attribute [-instance] WType.instEncodableWType Encodable.finPi Encodable.fintype
 
 namespace WType
 
-section elimv
-
-variable {α σ γ : Type*} {β : α → Type*}
-
-def elimv (fs : σ → σ) (fγ : σ → (Σ a : α, β a → γ) → γ) : σ → WType β → γ
-  | x, ⟨a, f⟩ => fγ x ⟨a, fun b => elimv fs fγ (fs x) (f b)⟩
-
-lemma elimv_eq_elim {fγ : σ → (Σ a : α, β a → γ) → γ} : elimv id fγ a = elim γ (fγ a) := by
-  funext w; induction' w with a f ih; simp[elim, elimv, ih]
-
-lemma elimv_eq_elimv (fs : τ → σ → σ) (fγ : τ → σ → (Σ a : α, β a → γ) → γ) (x z) :
-    elimv (fs x) (fγ x) z = elimv (fun (p : τ × σ) => (p.1, fs p.1 p.2)) (fun (p : τ × σ) => fγ p.1 p.2) (x, z) := by
-  funext w; induction w generalizing x z; simp[elimv, *]
-
-end elimv
-
 open Encodable Primrec Primcodable UniformlyPrimcodable
 variable {α : Type*} {β : α → Type*}
   [Primcodable α] [(a : α) → Fintype (β a)] [(a : α) → DecidableEq (β a)] [(a : α) → Primcodable (β a)] [PrimrecCard β]
+
+def inversion : WType β → α × List (WType β)
+  | ⟨a, f⟩ => ⟨a, List.ofFn $ fintypeArrowEquivFinArrow f⟩
+
+def elimv {σ γ : Type*} (fs : α → σ → σ) (fγ : σ → (Σ a : α, β a → γ) → γ) : σ → WType β → γ
+  | x, ⟨a, f⟩ => fγ x ⟨a, fun b => elimv fs fγ (fs a x) (f b)⟩
 
 def elimOpt (γ : Type*) (fγ : (Σ a : α, β a → γ) → Option γ) : WType β → Option γ
   | ⟨a, f⟩ => (toFinArrowOpt (fun b => elimOpt γ fγ (f b))).bind fun g => fγ ⟨a, g⟩
@@ -33,7 +23,22 @@ def SubWType {α : Type*} (β : α → Type*)
 
 namespace SubWType
 
+@[ext] lemma ext (w₁ w₂ : SubWType β s) : w₁.val = w₂.val → w₁ = w₂ := by
+  rcases w₁ with ⟨w₁, h₁⟩
+  rcases w₂ with ⟨w₂, h₂⟩
+  simp; rintro rfl; apply Subtype.ext (by simp)
+
+def cast {s'} (hs : s = s') (w : SubWType β s) : SubWType β s' := ⟨w.val, by simp[←hs]; exact w.prop⟩
+
+@[simp] def cast_refl (h : s = s) (w : SubWType β s) : cast h w = w := rfl
+
 def mk (a : α) (f : β a → SubWType β s) : SubWType β (s + 1) := ⟨⟨a, fun i => (f i).val⟩, by simp[depth]; intro b; exact (f b).property ⟩
+
+@[simp] lemma cast_mk {s'} (hs : s + 1 = s' + 1) (a : α) (f : β a → SubWType β s) :
+  cast hs (mk a f) = mk a (fun i => cast (by apply Nat.succ_inj'.mp hs) (f i)) := rfl
+
+@[simp] lemma cast_mk_one (hs : s + 1 = 1) (a : α) (f : β a → SubWType β s) :
+  cast hs (mk a f) = mk a (fun i => cast (by apply Nat.succ_inj'.mp hs) (f i)) := rfl
 
 abbrev ofWType (w : WType β) (n) (h : w.depth ≤ n) : SubWType β n := ⟨w, h⟩
 
@@ -59,19 +64,6 @@ def equiv_succ : SubWType β (n + 1) ≃ (Σ a : α, β a → SubWType β n) whe
   invFun := fun ⟨a, f⟩ => ofWType (WType.mk a (fun b => (f b).val)) (n + 1) (by simp[depth])
   left_inv := fun ⟨t, h⟩ => by rcases t with ⟨a, f⟩; simp
   right_inv := fun ⟨a, f⟩ => by simp
-
-def elimv' {σ : Type*} {γ : Type*} (fs : σ → σ) (fγ : σ → (Σ a : α, β a → γ) → γ) (s) :
-    σ → SubWType β s → γ := fun x ⟨t, _⟩ => t.elimv fs fγ x
-
-lemma elimv_const {w₁ : SubWType β s₁} {w₂ : SubWType β s₂} (h : w₁.val = w₂.val) (γ) (fγ : (Σ a : α, β a → γ) → γ) : 
-    elim' γ fγ s₁ w₁ = elim' γ fγ s₂ w₂ := by
-  rcases w₁ with ⟨w, hw₁⟩
-  rcases w₂ with ⟨w, hw₂⟩
-  simp at h; rcases h with rfl
-  simp[elim']
-
-lemma elimv'_eq_elim' {fγ : σ → (Σ a : α, β a → γ) → γ} (s) : elimv' id fγ s a = elim' γ (fγ a) s := by
-  funext ⟨w, _⟩; simp[elim', elimv', elimv_eq_elim]
 
 def primcodable_zero : Primcodable (SubWType β 0) := Primcodable.ofEquiv _ equiv_zero
 
@@ -114,6 +106,9 @@ lemma encode_mk (a : α) (f : β a → WType β) (h) :
   rw[Encodable.encode_sigma_val]
   simp; exact encode_fintypeArrow' (β a) (SubWType β s) _
 
+lemma encode_cast (w : SubWType β s) {s'} (hs : s = s') : encode w = encode (cast hs w) := by
+  rcases hs with rfl; simp
+
 section elimDecode
 
 variable {σ : Type*} {γ : Type*}
@@ -122,89 +117,82 @@ variable (β)
 def elimDecode (f : α → List γ → γ) : ℕ → ℕ → Option γ :=
  fun s e => (decode e : Option (SubWType β s)).map (elim' γ (fun ⟨a, v⟩ => f a (List.ofFn $ fintypeArrowEquivFinArrow v)) s)
 
-def elimvDecode (fs : σ → σ) (f : σ → α → List γ → γ) : σ → ℕ → ℕ → Option γ :=
- fun x s e => (decode e : Option (SubWType β s)).map
-   (elimv' fs (fun x ⟨a, v⟩ => f x a (List.ofFn $ fintypeArrowEquivFinArrow v)) s x)
-
-lemma elimvDecode_eq_induction (fs : σ → σ) (f : σ → α → List γ → γ) (x s e) :
-    elimvDecode β fs f x s e =
+lemma elimDecode_eq_induction (f : α → List γ → γ) (s e) :
+    elimDecode β f s e =
     Nat.casesOn s none
       (fun s => (decode e.unpair.1 : Option α).bind
-        $ fun a => (((Denumerable.ofNat (List ℕ) e.unpair.2).mapM' (elimvDecode β fs f (fs x) s)).bind
+        $ fun a => (((Denumerable.ofNat (List ℕ) e.unpair.2).mapM' (elimDecode β f s)).bind
           $ fun l => if l.length = Fintype.card (β a) then some l else none).map
-            $ fun v => f x a v) := by
+            $ fun v => f a v) := by
   rcases s with (_ | s)
-  · simp[elimvDecode]
-  · simp[elimvDecode, SubWType.decode_succ, Option.map_bind', decode_list, Function.comp, List.mapM'_option_map]; congr
+  · simp[elimDecode]
+  · simp[elimDecode, SubWType.decode_succ, Option.map_bind', decode_list, Function.comp, List.mapM'_option_map]; congr
     funext a
     rcases hw : List.mapM' (decode : ℕ → Option (SubWType β s)) (Denumerable.ofNat (List ℕ) e.unpair.2) with (_ | w) <;> simp
     { simp[List.toVector]
-      by_cases hlw : w.length = Fintype.card (β a) <;> simp[hlw, elimv, elimv']
+      by_cases hlw : w.length = Fintype.card (β a) <;> simp[hlw, elim, elim']
       { simp[Vector.get_mk_eq_get, List.ofFn_get_eq_map]; congr
-        rw[Encodable.fintypeArrowEquivFinArrow_fintypeEquivFin (fun i => WType.elimv fs _ (fs x) (w.get (i.cast hlw.symm)).val),
-          List.ofFn_get_eq_map (fun z => WType.elimv fs _ (fs x) z.val) w]; rfl } }
+        rw[Encodable.fintypeArrowEquivFinArrow_fintypeEquivFin (fun i =>
+          WType.elim γ (fun x => f x.fst (List.ofFn (fintypeArrowEquivFinArrow x.snd))) (w.get (i.cast hlw.symm)).val)];
+        rw[List.ofFn_get_eq_map (fun z => WType.elim γ (fun x => f x.fst (List.ofFn (fintypeArrowEquivFinArrow x.snd))) z.val) w];rfl } }
 
 @[reducible]
-private def elimvDecodeG (f : α → List γ → γ) : ℕ × ℕ → List (Option γ) → Option γ := fun (s, e) ih =>
+private def elimDecodeG (f : σ → α → List γ → γ) : σ → ℕ × ℕ → List (Option γ) → Option γ := fun x (s, e) ih =>
   Nat.casesOn s none
-    (fun _ => (decode e.unpair.1 : Option α).bind
-      $ fun a => (((Denumerable.ofNat (List ℕ) e.unpair.2).mapM' (fun c => ih.getI c)).bind
+    (fun s => (decode e.unpair.1 : Option α).bind
+      $ fun a => (((Denumerable.ofNat (List ℕ) e.unpair.2).mapM' (fun c => ih.getI (s.pair c))).bind
         $ fun l => if l.length = Fintype.card (β a) then some l else none).map
-          $ fun v => f a v)
+          $ fun v => f x a v)
 
-private lemma elimvDecodeG_eq_elimvDecode (fs : σ → σ) (f : σ → α → List γ → γ) (x s e) :
-    elimvDecodeG β (f x) (s, e) ((List.range e).map (elimvDecode β fs f (fs x) s.pred)) =
-    elimvDecode β fs f x s e := by
-  simp[elimvDecode_eq_induction β fs f x s e, elimvDecodeG]
+private lemma elimDecodeG_eq_elimDecode (f : σ → α → List γ → γ) (x s e) :
+    elimDecodeG β f x (s, e) ((List.range (s.pair e)).map (fun i => elimDecode β (f x) i.unpair.1 i.unpair.2)) = elimDecode β (f x) s e := by
+  simp[elimDecode_eq_induction β (f x) s e, elimDecodeG]
   rcases s with (_ | s) <;> simp; congr
   funext a
-  have : mapM' (fun c => ((List.range e).map $ elimvDecode β fs f (fs x) s).getI c)
+  have : 
+    mapM' (fun c => ((List.range ((s + 1).pair e)).map $ fun i => elimDecode β (f x) i.unpair.fst i.unpair.snd).getI (s.pair c))
       (Denumerable.ofNat (List ℕ) e.unpair.2) =
-    mapM' (elimvDecode β fs f (fs x) s) (Denumerable.ofNat (List ℕ) e.unpair.2) :=
+    mapM' (elimDecode β (f x) s) (Denumerable.ofNat (List ℕ) e.unpair.2) :=
   List.mapM'_eq_mapM'_of_eq _ (by
   { intro c hc
-    have : c < e := by
+    have : s.pair c < (s + 1).pair e := by
       have : c < e.unpair.2 := Denumerable.lt_of_mem_list _ _ hc
-      exact lt_of_lt_of_le this (Nat.unpair_right_le e)
+      exact lt_of_lt_of_le (Nat.pair_lt_pair_right s this) (Nat.pair_le_pair_of_le (Nat.le_succ s) (Nat.unpair_right_le e))
     simp[List.getI_map_range _ this] })
   rw[this]
 
 variable [Primcodable σ] [Primcodable γ]
 
-private lemma elimvDecodeG_primrec {f : σ → α × List γ → γ} (hf : Primrec₂ f) :
-    Primrec₂ (fun p ih => elimvDecodeG β (fun a ih => f p.1.1 (a, ih)) (p.1.2, p.2) ih
-      : (σ × ℕ) × ℕ → List (Option γ) → Option γ) :=
-  to₂' <| nat_casesOn (snd.comp $ fst.comp fst) (const _)
-    <| to₂' <| option_bind
-      (Primrec.decode.comp $ fst.comp $ unpair.comp $ snd.comp $ fst.comp fst)
+private lemma elimDecodeG_primrec {f : σ → α × List γ → γ} (hf : Primrec₂ f) :
+    Primrec₂ (fun p ih => elimDecodeG β (fun x a ih => f x (a, ih)) p.1 p.2 ih : σ × (ℕ × ℕ) → List (Option γ) → Option γ) :=
+  to₂' <| Primrec.nat_casesOn (fst.comp $ snd.comp fst) (const none)
+    <| to₂' <| option_bind (Primrec.decode.comp $ fst.comp $ unpair.comp $ snd.comp $ snd.comp $ fst.comp fst)
       <| to₂' <| option_map
         (option_bind
           (option_list_mapM'
-            ((Primrec.ofNat _).comp $ snd.comp $ unpair.comp $ snd.comp $ fst.comp $ fst.comp fst)
-            (list_getI.comp₂ (snd.comp₂ $ fst.comp₂ $ fst.comp₂ Primrec₂.left) Primrec₂.right))
-          (to₂' $ Primrec.ite
+            ((Primrec.ofNat _).comp $ snd.comp $ unpair.comp $ snd.comp $ snd.comp $ fst.comp $ fst.comp $ fst)
+            (to₂' <| list_getI.comp (snd.comp $ fst.comp $ fst.comp fst)
+              (Primrec₂.natPair.comp (snd.comp $ fst.comp fst) snd)))
+          (to₂' <| Primrec.ite
             (Primrec.eq.comp (list_length.comp snd) (PrimrecCard.card_prim.comp $ snd.comp fst))
-            (option_some.comp snd) (const _)))
-        (hf.comp₂ (fst.comp₂ $ fst.comp₂ $ fst.comp₂ $ fst.comp₂ $ fst.comp₂ $ Primrec₂.left)
-          (Primrec₂.pair.comp₂ (snd.comp₂ Primrec₂.left) Primrec₂.right))
+            (option_some.comp snd)
+            (const none)))
+        (to₂' <| hf.comp (fst.comp $ fst.comp $ fst.comp $ fst.comp fst) (Primrec.pair (snd.comp fst) snd))
 
-lemma primrec_elimvDecode {fs : σ → σ} {f : σ → α × List γ → γ} (hfs : Primrec fs) (hf : Primrec₂ f) :
-    Primrec₂ (fun x p => elimvDecode β fs (fun x a ih => f x (a, ih)) x p.1 p.2 : σ → ℕ × ℕ → Option γ) := by
-  let F : σ × ℕ → ℕ → Option γ := (fun p e => elimvDecode β fs (fun x a ih => f x (a, ih)) p.1 p.2 e)
-  have := nat_one_side_strong_rec F (option_some.comp₂ (elimvDecodeG_primrec β hf))
-    (Primrec₂.pair.comp (hfs.comp fst) (pred.comp snd))
-    (fun (x, s) e => by
-      simpa using elimvDecodeG_eq_elimvDecode β fs (fun x a ih => f x (a, ih)) x s e)
-  exact this.comp₂ (Primrec₂.pair.comp₂ Primrec₂.left (fst.comp₂ Primrec₂.right)) (snd.comp₂ Primrec₂.right)
+lemma primrec_elimDecode_param {f : σ → α × List γ → γ} (hf : Primrec₂ f) :
+    Primrec₂ (fun x p => elimDecode β (fun a ih => f x (a, ih)) p.1 p.2 : σ → ℕ × ℕ → Option γ) := by
+  have : Primrec₂ (fun p ih => some $ elimDecodeG β (fun x a ih => f x (a, ih)) p.1 p.2 ih : σ × (ℕ × ℕ) → List (Option γ) → Option (Option γ)) :=
+    option_some.comp (elimDecodeG_primrec β hf)
+  exact nat_strong_rec'2 _ this (by simp[elimDecodeG_eq_elimDecode β])
 
 lemma primrec_elimDecode {f : α → List γ → γ} (hf : Primrec₂ f) :
-    Primrec₂ (fun s e => elimDecode β f s e : ℕ → ℕ → Option γ) := by
-  have : Primrec₂ (fun _ p => f p.1 p.2 : Unit → α × List γ → γ) :=
-    hf.comp₂ (fst.comp₂ Primrec₂.right) (snd.comp₂ Primrec₂.right)
-  have H := primrec_elimvDecode β (fs := (id : Unit → Unit)) Primrec.id this
-  have : Primrec₂ (fun _ e => (e, ()) : ℕ → ℕ → ℕ × Unit) := (Primrec₂.pair.comp₂ Primrec₂.right (Primrec₂.const ()))
-  exact (H.comp₂ (Primrec₂.const ()) (Primrec₂.pair.comp₂ Primrec₂.left Primrec₂.right)).of_eq <|
-    by intro s e; simp[elimvDecode, elimDecode, elimv'_eq_elim']
+    Primrec₂ (fun s e => elimDecode β f s e : ℕ → ℕ → Option γ) :=
+  have : Primrec₂ (fun _ p => f p.1 p.2 : Unit → α × List γ → γ) := hf.comp (fst.comp snd) (snd.comp snd)
+  (primrec_elimDecode_param β this).comp₂ (const ()).to₂ (fst.pair snd)
+
+lemma primrec_elimDecode_param_comp {f : σ → α × List γ → γ} {g : σ → ℕ} {h : σ → ℕ} (hf : Primrec₂ f) (hg : Primrec g) (hh : Primrec h) :
+    Primrec (fun x => elimDecode β (fun a l => f x (a, l)) (g x) (h x) : σ → Option γ) :=
+  (primrec_elimDecode_param β hf).comp Primrec.id (hg.pair hh)
 
 end elimDecode
 
@@ -273,8 +261,8 @@ private lemma primrec_encode_decode :
         $ fun c => ((decode c : Option (SubWType β e.unpair.1)).map (fun w => w.val.depth)).map
           $ fun d => d.pair c)) : ℕ → ℕ) :=
   (Primrec.encode.comp $
-    option_bind (Primrec₂.encodeDecode_u.comp (fst.comp Primrec.unpair) (snd.comp Primrec.unpair))
-      (option_map (SubWType.depth_decode_primrec.comp (fst.comp $ Primrec.unpair.comp fst) snd)
+    option_bind (Primrec₂.encodeDecode_u.comp (fst.comp unpair) (snd.comp unpair))
+      (option_map (SubWType.depth_decode_primrec.comp (fst.comp $ unpair.comp fst) snd)
         (Primrec₂.natPair.comp₂ Primrec₂.right (snd.comp fst))))
 
 private def encodable : Encodable (WType β) where
@@ -293,15 +281,8 @@ lemma decode_eq (e : ℕ) : decode e = (decode e : Option ((s : ℕ) × SubWType
 def elimL (f : α → List γ → γ) : WType β → γ :=
   elim γ (fun ⟨a, v⟩ => f a (List.ofFn $ fintypeArrowEquivFinArrow v))
 
-def elimvL (fs : σ → σ) (f : σ → α → List γ → γ) : σ → WType β → γ :=
-  elimv fs (fun x ⟨a, v⟩ => f x a (List.ofFn $ fintypeArrowEquivFinArrow v))
-
 lemma elimL_mk (f : α → List γ → γ) (a : α) (v : β a → WType β) :
     elimL f ⟨a, v⟩ = f a (List.ofFn $ fintypeArrowEquivFinArrow $ fun b => elimL f (v b)) := by simp[elimL, elim]
-
-lemma elimvL_mk (fs : σ → σ) (f : σ → α → List γ → γ) (a : α) (v : β a → WType β) :
-    elimvL fs f x ⟨a, v⟩ = f x a (List.ofFn $ fintypeArrowEquivFinArrow $ fun b => elimvL fs f (fs x) (v b)) := by
-  simp[elimvL, elimv]
 
 lemma elim_eq_elimL [Inhabited γ] (f : (a : α) × (β a → γ) → γ) :
     elim γ f w = elimL (fun a l => f ⟨a, fintypeArrowEquivFinArrow.symm (fun i => l.getI i)⟩) w := by
@@ -312,10 +293,11 @@ lemma decode_elimL_eq (f : α → List γ → γ) :
   simp[elimL, decode_eq, Function.comp, SubWType.elimDecode, SubWType.elim']
   rcases (decode e.unpair.2) with (_ | ⟨_, _⟩) <;> simp[SubWType.toW]
 
-lemma decode_elimvL_eq (fs : σ → σ) (f : σ → α → List γ → γ) :
-    (decode e : Option (WType β)).map (elimvL fs f x) = (SubWType.elimvDecode β fs f x e.unpair.1 e.unpair.2) := by
-  simp[elimvL, decode_eq, Function.comp, SubWType.elimvDecode, SubWType.elimv']
-  rcases (decode e.unpair.2) with (_ | ⟨_, _⟩) <;> simp[SubWType.toW]
+def elimvL (fs : α → σ → σ) (fγ : σ → α → List γ → γ) : σ → WType β → γ :=
+  elimv fs (fun x ⟨a, v⟩ => fγ x a (List.ofFn $ fintypeArrowEquivFinArrow v))
+
+lemma elimvL_mk (fs : α → σ → σ) (fγ : σ → α → List γ → γ) (a : α) (v : β a → WType β) :
+    elimvL fs fγ x ⟨a, v⟩ = fγ x a (List.ofFn $ fintypeArrowEquivFinArrow $ fun b => elimvL fs fγ (fs a x) (v b)) := by simp[elimvL, elimv]
 
 def mkL (a : α) (l : List (WType β)) : Option (WType β) :=
   if h : l.length = Fintype.card (β a) then
@@ -337,6 +319,11 @@ lemma encode_mk_eq (a : α) (f : β a → WType β) :
 lemma mk₀_eq (a : α) [h : IsEmpty (β a)] : mk₀ a = some (⟨a, h.elim'⟩ : WType β) := by
   simp[mk₀, mkL, Fintype.card_eq_zero_iff.mpr h]
 
+lemma mkL_inversion (w : WType β) : mkL (inversion w).1 (inversion w).2 = w := by
+  rcases w with ⟨a, f⟩
+  simp[inversion, mkL, Fin.castIso_eq_cast]
+  funext; simp
+
 end WType
 
 namespace Primrec
@@ -346,9 +333,9 @@ variable {τ σ α γ : Type*} {β : α → Type*}
   [Primcodable τ] [Primcodable σ] [Primcodable α] [(a : α) → Fintype (β a)]
   [(a : α) → DecidableEq (β a)] [(a : α) → Primcodable (β a)] [PrimrecCard β] [Primcodable γ]
 
-lemma w_depth : Primrec (fun w => w.depth : WType β → ℕ) := by
+lemma w_depth : Primrec (depth : WType β → ℕ) := by
   have : Primrec (fun n => (encodeDecode (WType β) n).map $ fun e => e.unpair.1) :=
-    option_map Primrec.encodeDecode (fst.comp₂ $ Primrec.unpair.comp₂ Primrec₂.right)
+    option_map Primrec.encodeDecode (fst.comp₂ $ unpair.comp₂ Primrec₂.right)
   exact decode_iff.mp (this.of_eq $ fun n => by
     simp[encodeDecode_eq_encode_map_decode]
     rcases decode n <;> simp[WType.encode_eq, WType.SubWType.ofW])
@@ -356,35 +343,14 @@ lemma w_depth : Primrec (fun w => w.depth : WType β → ℕ) := by
 lemma w_elimL {f : α → List γ → γ} (hf : Primrec₂ f) : Primrec (elimL f : WType β → γ) :=
   decode_iff.mp (by simp[decode_elimL_eq]; apply SubWType.primrec_elimDecode β hf)
 
-lemma w_elimvL {fs : σ → σ} {f : σ → α × List γ → γ}
-  (hfs : Primrec fs) (hf : Primrec₂ f) : Primrec₂ (elimvL fs (fun x a v => f x (a, v)) : σ → WType β → γ) :=
-  Primrec₂.decode_iff₂.mp (by
-    simp[decode_elimvL_eq]
-    exact (SubWType.primrec_elimvDecode β hfs hf).comp₂ Primrec₂.left
-      (Primrec₂.pair.comp₂
-        (fst.comp₂ $ unpair.comp₂ Primrec₂.right)
-        (snd.comp₂ $ unpair.comp₂ Primrec₂.right)))
-
-lemma w_elimvL_param {fs : τ → σ → σ} {f : τ → σ × (α × List γ) → γ} {s : τ → σ} {g : τ → WType β}
-  (hfs : Primrec₂ fs) (hf : Primrec₂ f) (hs : Primrec s) (hg : Primrec g) :
-    Primrec (fun x => elimvL (fs x) (fun z a l => f x (z, a, l)) (s x) (g x)) := by
-  have := (w_elimvL (β := β)
-      (Primrec₂.pair.comp fst (hfs.comp fst snd))
-      (hf.comp₂ (fst.comp₂ Primrec₂.left) (Primrec₂.pair.comp₂ (snd.comp₂ Primrec₂.left) Primrec₂.right))).comp
-    (Primrec₂.pair.comp Primrec.id hs) hg
-  apply this.of_eq <| by
-    intro x; simp[elimvL]; apply congr_fun; exact Eq.symm <|
-      elimv_eq_elimv fs (fun x z (p : Σ a, β a → γ) => f x (z, p.1, List.ofFn $ fintypeArrowEquivFinArrow p.2)) x (s x)
-
--- TODO: delete
-lemma w_elimvL_param' {fs : τ → σ → σ} {f : τ → σ → α → List γ → γ} {s : τ → σ} {g : τ → WType β}
-  (hfs : Primrec₂ fs) (hf : Primrec₂ (fun (p : τ × σ) (q : α × List γ) => f p.1 p.2 q.1 q.2)) (hs : Primrec s) (hg : Primrec g) :
-    Primrec (fun x => elimvL (fs x) (f x) (s x) (g x)) := by
-  have := ((w_elimvL (β := β) (Primrec₂.pair.comp fst (hfs.comp fst snd)) hf)).comp
-    (Primrec₂.pair.comp Primrec.id hs) hg
-  exact this.of_eq <| by
-    intro x; simp[elimvL]; exact Eq.symm <|
-      congr_fun (elimv_eq_elimv fs (fun x z (p : Σ a, β a → γ) => f x z p.1 (List.ofFn $ fintypeArrowEquivFinArrow p.2)) x (s x)) _
+lemma w_elimL_param {f : σ → α × List γ → γ} {w : σ → WType β} (hf : Primrec₂ f) (hw : Primrec w) :
+    Primrec (fun x => elimL (fun p l => f x (p, l)) (w x) : σ → γ) := by
+  have : Primrec₂ (fun x w => elimL (fun p l => f x (p, l)) w : σ → WType β → γ) :=
+  Primrec₂.decode_iff₂.mp
+    (by simp[decode_elimL_eq]
+        exact (SubWType.primrec_elimDecode_param β hf).comp₂ Primrec₂.left
+          (Primrec.pair (fst.comp $ Primrec.unpair.comp snd) (snd.comp $ Primrec.unpair.comp snd)).to₂)
+  exact this.comp Primrec.id hw
 
 lemma w_elim [Inhabited γ] {f : (a : α) × (β a → γ) → γ}
   (hf : Primrec₂ (fun a l => f ⟨a, fintypeArrowEquivFinArrow.symm (fun i => l.getI i)⟩ : α → List γ → γ)) :
@@ -455,5 +421,52 @@ lemma w_mkFin (f : σ → α) {k} (h : ∀ x, Fintype.card (β (f x)) = k) (hf :
     have := (fintypeArrowEquivFinArrow' (α := WType β) (h x)).injective
     apply this
     funext i; simp; congr)
+
+lemma w_inversion [Inhabited (WType β)] : Primrec (WType.inversion : WType β → α × List (WType β)) := by
+  have : Primrec₂ (fun a l => (a, l.map (fun p => (mkL p.1 p.2).get!)) : α → List (α × List (WType β)) → α × List (WType β)) :=
+    Primrec₂.pair.comp₂ Primrec₂.left
+      (to₂' <| list_map snd (option_get!.comp₂ $ w_mkL.comp₂ (fst.comp₂ $ Primrec₂.right) (snd.comp₂ $ Primrec₂.right)))
+  have := w_elimL (β := β) this
+  exact this.of_eq <| fun w => by
+    induction w
+    simp[inversion, elimL_mk, Function.comp]
+    funext i; simp[*, mkL_inversion]
+
+lemma w_elimvL_param [Inhabited (WType β)] {fs : τ → α × σ → σ} {fγ : τ → σ × α × List γ → γ} {g : τ → σ} {w : τ → WType β}
+  (hfs : Primrec₂ fs) (hfγ : Primrec₂ fγ) (hg : Primrec g) (hw : Primrec w) :
+    Primrec (fun z => WType.elimvL (fun a x => fs z (a, x)) (fun x a l => fγ z (x, a, l)) (g z) (w z)) := by
+  have : Primrec₂ (fun z (p : σ × WType β) => WType.elimvL (fun a x => fs z (a, x)) (fun x a l => fγ z (x, a, l)) p.1 p.2) :=
+    to₂' <| by {
+      have hm : Primrec (fun (p : τ × σ × WType β) => p.2.2.depth) := w_depth.comp <| snd.comp snd
+      have hl : Primrec (fun (p : τ × σ × WType β) =>
+          p.2.2.inversion.2.map (fun w => (p.1, fs p.1 (p.2.2.inversion.1, p.2.1), w))) :=
+        list_map (snd.comp $ w_inversion.comp $ snd.comp snd)
+          <| Primrec₂.pair.comp (fst.comp fst)
+          <| Primrec₂.pair.comp
+            (hfs.comp (fst.comp fst)
+              (Primrec₂.pair.comp
+                (fst.comp $ w_inversion.comp $ snd.comp $ snd.comp fst)
+                (fst.comp $ snd.comp fst)))
+          <| snd
+      have hg : Primrec₂ (fun (p : τ × σ × WType β) (l : List γ) => fγ p.1 (p.2.1, p.2.2.inversion.1, l)) :=
+        hfγ.comp₂ (fst.comp₂ Primrec₂.left)
+          <| Primrec₂.pair.comp₂ (fst.comp₂ $ snd.comp₂ Primrec₂.left)
+          <| Primrec₂.pair.comp₂ (fst.comp₂ $ w_inversion.comp₂ $ snd.comp₂ $ snd.comp₂ Primrec₂.left) Primrec₂.right
+      apply strong_rec _ hm hl (option_some.comp₂ hg)
+        (by rintro ⟨z, x, ⟨a, f⟩⟩ ⟨z', x', w'⟩
+            simp[inversion, Function.comp, List.mem_ofFn]
+            rintro rfl rfl i rfl; exact depth_lt_depth_mk _ _ _)
+        (by { rintro ⟨z, x, ⟨a, f⟩⟩; simp[inversion, Function.comp, elimvL_mk]
+              congr }) }
+  exact this.comp Primrec.id (Primrec₂.pair.comp hg hw)
+
+lemma w_elimvL [Inhabited (WType β)] {fs : α → σ → σ} {fγ : σ → α × List γ → γ}
+  (hfs : Primrec₂ fs) (hfγ : Primrec₂ fγ) : Primrec₂ (WType.elimvL (β := β) fs (fun x a l => fγ x (a, l))) := to₂' <| by {
+  have hfs : Primrec₂ (fun _ p => fs p.1 p.2 : σ × WType β → α × σ → σ) :=
+    hfs.comp₂ (fst.comp₂ Primrec₂.right) (snd.comp₂ Primrec₂.right)
+  have hfγ : Primrec₂ (fun _ p => fγ p.1 p.2 : σ × WType β → σ × α × List γ → γ) :=
+    hfγ.comp₂ (fst.comp₂ Primrec₂.right) (snd.comp₂ Primrec₂.right)
+  exact w_elimvL_param hfs hfγ fst snd }
+  
 
 end Primrec
